\documentclass[a4paper,11pt,openany]{scrartcl}
\usepackage{../reg2021}
\usepackage{../quiver}

\begin{document}
\noindent\textbf{Author}\hfill\textbf{Semester} \linebreak
\vspace*{-.1cm} Matteo Durante, Yuhao Zhang\hfill WS 2020/21 \\

\noindent
\rule{\linewidth}{1pt}
\begin{center}
\Large
\textbf{Higher Category Theory} \\
Assignment 10
\end{center}
\rule{\linewidth}{1pt}
\\

%%%%%%%%%%%%%%%%%%%%%%%%%%%%%%%%%%%%%%%%%%%%%%%%%%%%%%%%%%%%%%%%%%%%%%%%%%%%%%%

%%%sheet4
\newcommand{\La}{\Lambda}
\newcommand{\pa}{\partial}
\newcommand{\ob}{\operatorname{Ob}}
\newcommand{\mor}{\operatorname{Mor}}
\newcommand{\sto}{\twoheadrightarrow}

%%%sheet5
\newcommand{\plim}{\varprojlim}
\newcommand{\sst}{\subseteq}
\newcommand{\eq}{\operatorname{eq}}

%%%sheet6
\newcommand{\f}{\varphi}

%%%sheet8
\newcommand{\sing}{\operatorname{Sing}}

%%%sheet9
\newcommand{\ihom}{\underline{\Hom}}


~\\
\exercise{1}

~\\
\exercise{2}
\begin{proof}
    (1) We begin by considering a commutative diagram
    \[\begin{tikzcd}
        {\Lambda^n_k} & {p^{-1}(a)=X_a} & X \\
        {\Delta^n} & {\Delta^0} & A
        \arrow["p", from=1-3, to=2-3]
        \arrow["a"', from=2-2, to=2-3]
        \arrow[from=1-2, to=1-3]
        \arrow[from=1-2, to=2-2]
        \arrow[from=2-1, to=2-2]
        \arrow[from=1-1, to=2-1]
        \arrow[from=1-1, to=1-2]
        \arrow[dotted, from=2-1, to=1-3]
        \arrow[dotted, from=2-1, to=1-2]
        \arrow["\lrcorner"{anchor=center, pos=0.01}, draw=none, from=1-2, to=2-3]
    \end{tikzcd},\]
    where $0\leq k<n$ and the square on the right is a pullback. From the LLP of
    $\Lambda^n_k\rightarrow\Delta^n$ against $p$ we get a lift
    $\Delta^n\rightarrow X$ and then, using the universal property of the
    pullback with respect to the lift and $\Delta^n\rightarrow\Delta^0$, we get
    a lift of $\Lambda^n_k\rightarrow\Delta^n$ against $X_a\rightarrow\Delta^0$.

    This implies that $X_a$ is an $\infty$-category, hence we only need to prove
    that its morphisms are invertible, which will make it a $\infty$-groupoid
    and therefore a Kan complex.

    To prove this, for any morphism $f\colon x\rightarrow y$ in $X_a$ we
    consider the diagram
    \[\begin{tikzcd}
        {\Lambda^2_0} & {X_a} \\
        {\Delta^2}
        \arrow["{(\id_x,f)}", from=1-1, to=1-2]
        \arrow[from=1-1, to=2-1]
        \arrow["t"', dotted, from=2-1, to=1-2]
    \end{tikzcd}\]
    inducing the pictured 2-simplex $t$ by our previous observations. The
    morphism $f$ is a right inverse of $d_2(t)=g\colon y\rightarrow x$ and from
    \[\begin{tikzcd}
        {\Lambda^2_0} & {X_a} \\
        {\Delta^2}
        \arrow["{(\id_y,g)}", from=1-1, to=1-2]
        \arrow[from=1-1, to=2-1]
        \arrow["u"', dotted, from=2-1, to=1-2]
    \end{tikzcd}\]
    we also get a left inverse $d_2(u)=h$ of $g$. It follows that $g$ is
    invertible and the same goes for $f$.

    (2) Let's consider for any morphism $f\colon a_0\rightarrow a_1$ in $A$ the
    commutative diagram
    \[\begin{tikzcd}
        {\Lambda^1_0=\Delta^0} & X \\
        {\Delta^1} & A
        \arrow["p", from=1-2, to=2-2]
        \arrow["f"', from=2-1, to=2-2]
        \arrow["{x_0}", from=1-1, to=1-2]
        \arrow[from=1-1, to=2-1]
        \arrow["{\phi}"{description}, dotted, from=2-1, to=1-2]
    \end{tikzcd},\]
    which from the LLP of $\Lambda^1_0\rightarrow\Delta^1$ against $p$ grants us
    the desired lift $\phi\colon x_0\rightarrow x_1$ of $f$ along $p$.

    To prove that the equivalence class of $x_1$ in $\pi_0(X_{a_1})$ does not
    depend on the choice of the lift we consider for any other such lift
    $\psi\colon x_0\rightarrow y$ the commutative diagram
    \[\begin{tikzcd}
        {\Lambda^2_0} & X \\
        {\Delta^2} & A
        \arrow["{s_0(f)}"', from=2-1, to=2-2]
        \arrow["{(\psi,\phi)}", from=1-1, to=1-2]
        \arrow["p", from=1-2, to=2-2]
        \arrow[from=1-1, to=2-1]
        \arrow["t"{description}, dotted, from=2-1, to=1-2]
    \end{tikzcd},\]
    granting us a 2-simplex $t$ which induces a morphism $d_0(t)=\xi\colon
    x_1\rightarrow y$. The commutative diagram
    \[\begin{tikzcd}
        {\Delta^1} \\
        & {X_a} & X \\
        & {\Delta^0} & A
        \arrow[curve={height=6pt}, from=1-1, to=3-2]
        \arrow["\xi", curve={height=-6pt}, from=1-1, to=2-3]
        \arrow["\xi"{description}, dotted, from=1-1, to=2-2]
        \arrow[from=2-2, to=3-2]
        \arrow["{a_1}", from=3-2, to=3-3]
        \arrow["p", from=2-3, to=3-3]
        \arrow[from=2-2, to=2-3]
        \arrow["\lrcorner"{anchor=center, pos=0.01}, draw=none, from=2-2, to=3-3]
    \end{tikzcd}\]
    then shows that this morphism also lies in $X_a$ through the universal
    property of the pullback and therefore $[x_1]=[y]$ in $\pi_0(X_a)$.

    We have just proven that distinct lifts through $p$ of the same morphism
    have the same codomain up to equivalence as long as they have the same
    domain.

    (3) Let $t\colon\Delta^2\rightarrow A$ be the map corresponding to our
    commutative trangle. We proceed by drawing the commutative diagram
    \[\begin{tikzcd}
        {\Lambda^2_1} & X \\
        {\Delta^2} & A
        \arrow["t"', from=2-1, to=2-2]
        \arrow["p", from=1-2, to=2-2]
        \arrow["{(\phi',\phi)}", from=1-1, to=1-2]
        \arrow[from=1-1, to=2-1]
        \arrow["u"{description}, dotted, from=2-1, to=1-2]
    \end{tikzcd},\]
    which by the LLP of $\Lambda^2_0\rightarrow\Delta^2$ against $p$ grants us a
    lift $u\colon\Delta^2\rightarrow X$ (and therefore a commutative triangle)
    with $d_0(u)=\phi'$, $d_1(u)=\psi\colon x_0\rightarrow x_2$ and
    $d_2(u)=\phi$ such that $p(\psi)=g$.

    (4) The functor, which we will denote by $F$, has already been well defined
    on objects, hence we only need to specify the action on morphisms. We know
    that for any map $f\colon a_0\rightarrow a_1$ in $A$ we have a lift
    $\phi\colon x_0\rightarrow x_1$ such that $p(\phi)=f$, thus we define
    $F([f])\colon\pi_0(X_{a_0})\rightarrow\pi_0(X_{a_1})$ as
    $F([f])([x_0])=[x_1]$, where $[x_1]$ lies in $\pi_0(X_{a_1})$ since
    $p(d_0(\phi))=d_0(p(\phi))=d_0(f)=a_1$.
    We need to show that this map is well defined, for which we will start with
    proving that, after fixing a representative $f$ of $[f]$, if we have a
    morphism $\psi\colon x_0\rightarrow x_0'$ in $X_{a_0}$ then we also have a
    morphism $x_1\rightarrow x_1'$ in $X_{a_1}$ between the objects specified by
    the liftings $\phi$, $\phi'$ of $f$ with domains $x_0$, $x_0'$.

    We can construct a map
    $(\phi'\cdot\psi,\phi)\colon\Lambda^2_0\rightarrow X$ which, composed
    with $p$, gives us $(p(\phi'\cdot\psi),f)\colon\Lambda^2_0\rightarrow A$. We
    want to extend this to a $2$-simplex $t\colon\Delta^2\rightarrow A$ where
    $d_0(t)=\id_a$; we will then lift it through $p$ thanks to the RLP with
    respect to $\Lambda^2_0\rightarrow\Delta^2$, getting a 2-simplex $t'$ in $X$
    such that $d_0(t')$ will be by construction the desired morphism
    $x_1\rightarrow x_1'$ in $X_{a_1}$.

    Notice that we have 2-simplices $u$, $v$ showing that $p(\phi'\cdot\psi)\sim
    p(\phi')\cdot p(\psi)=f\cdot\id_a$, $f=f\cdot\id_a$, thus we may construct
    a horn $(s_0(f),v,u)\colon\Lambda^3_1\rightarrow A$ giving us a 3-simplex
    $\alpha$ such that $t=d_1(\alpha)$ is the desired 2-simplex in $A$.

    Having proven that $F([f])([x_0])$ does not depend on the representative of
    $[x_0]$, we show that it also does not depend on the representative of
    $[f]$.

    Suppose that $g\in [f]$, i.e.\ we have a 2-simplex $t$ in $A$ showing that
    $\id_a\cdot f\sim g$, meaning that $d_0(t)=\id_a$, $d_1(t)=g$, $d_2(t)=f$.
    After choosing lifts $\phi\colon x_0\rightarrow x_1$, $\psi\colon
    x_0\rightarrow x_1'$ of $f$, $g$ through $p$, we can construct the
    commutative square
    \[\begin{tikzcd}
        {\Lambda^2_0} & X \\
        {\Delta^2} & A
        \arrow["{(\psi,\phi)}", from=1-1, to=1-2]
        \arrow[from=1-1, to=2-1]
        \arrow["t"', from=2-1, to=2-2]
        \arrow["p", from=1-2, to=2-2]
        \arrow["u"{description}, dotted, from=2-1, to=1-2]
    \end{tikzcd},\]
    where the lift $u$ is such that $d_0(u)=h$ provides the desired morphism
    $x_1\rightarrow x_1'$ in $X_{a_1}$.

    This shows that $F([f])$ is well defined. We still have to prove that this
    association is functorial.

    If $[f]=[\id_a]$, then for any $[x]\in\pi_0(X_a)$ we may pick $\id_x$ as a
    lift of $\id_a$ through $p$, which then shows that $F([\id_a])([x])=[x]$.

    On the other hand, consider two composable morphisms $[f]$, $[g]$, where
    $\dom(f)=a$. Given a
    2-simplex $t$ in $A$ such that $d_0(t)=g$, $d_1(t)=g\cdot f$, $d_2(t)=f$ and
    fixed an element $[x_0]\in\pi_0(X_a)$, after fixing lifts $\phi\colon
    x_0\rightarrow x_1$, $\psi\colon x_1\rightarrow x_2$ of $f$, $g$ by (3) we
    get a 2-simplex $u$ in $X$
    such that $d_0(u)=\psi$, $d_1(u)=\xi\colon x_0\rightarrow x_2$,
    $d_2(u)=\phi$ and $\xi$ is a lift of $g\cdot f$ through $p$ with
    $\phi\cdot\psi\sim\xi$. It follows that $F([g]\cdot [f])=F([g])\cdot
    F([f])$.
\end{proof}

\end{document}
